Fixpoint; no induction principle

coq/two/LambdaTwo.v
@@ -1,39 +1,45 @@
 Require Export LambdaTwoSyntax.
 Require Export IndistinguishabilityTwo.
 
-
-Fixpoint eval L P pc e t a k {struct k} : Prop :=
-  match t, k with
-    | TNat n, 0 =>
+Fixpoint eval L P pc e t k a {struct k} :=
+  match t with
+    | TNat n =>
       a = Atom (VNat n) pc
-    | TVar n, 0 =>
+    | TVar n =>
       match atIndex e n with
         | Some (Atom v l) =>
           a = Atom v (l ⊔ pc)
         | None => False
       end
-    | TLam t', 0 =>
+    | TLam t' =>
       a = Atom (VClos e t') pc
-    | TApp t1 t2, S k' =>
-      forall e1' t1' l1 a2 a3,
-        eval L P pc e t1 (Atom (VClos e1' t1') l1) k' ->
-        eval L P pc e t2 a2 k' ->
-        eval L P l1 (a2 :: e1') t1' a3 k' ->
-        a = a3
-    | TDecl t1 t2, S k' =>
-      forall e1' t1' l1 a2 a3,
-        eval L P pc e t1 (Atom (VClos e1' t1') l1) k' ->
-        eval L P pc e t2 a2 k' ->
-        eval L P l1 (a2 :: e1') t1' a3 k' ->
-        match a3 with
-          | Atom v3 Bottom2 =>
+    | TApp t1 t2 =>
+      match k with
+        | S k' =>
+          forall e1' t1' l1 a2 a3,
+            eval L P pc e t1 k' (Atom (VClos e1' t1') l1) ->
+            eval L P pc e t2 k' a2 ->
+            eval L P l1 (a2 :: e1') t1' k' a3 ->
             a = a3
-          | Atom v3 Top2 =>
-            (forall a2' e2' v3',
-               env_LPequiv L P (a2 :: e1') (a2' :: e2') ->
-               eval L P l1 (a2' :: e2') t1' (Atom v3' Top2) k' ->
-               value_LPequiv L P v3 v3') ->
-            a = Atom v3 Bottom2
-        end
-    | _, _ => False
+        | 0 => False
+      end
+    | TDecl t1 t2 =>
+      match k with
+        | S k' =>
+          forall e1' t1' l1 a2 v3 l3,
+            eval L P pc e t1 k' (Atom (VClos e1' t1') l1) ->
+            eval L P pc e t2 k' a2 ->
+            eval L P l1 (a2 :: e1') t1' k' (Atom v3 l3) ->
+            match l3 with
+              | Bottom2 =>
+                a = (Atom v3 Bottom2)
+              | Top2 =>
+                (forall a2' e2' v3',
+                   env_LPequiv L P (a2 :: e1') (a2' :: e2') ->
+                   eval L P l1 (a2' :: e2') t1' k' (Atom v3' Top2) ->
+                   value_LPequiv L P v3 v3') ->
+                a = (Atom v3 Bottom2)
+            end
+        | 0 => False
+      end
   end.
