coq/two/LambdaTwoNI.v
@@ -7,47 +7,18 @@ Theorem non_interference_strong_observer :
   forall L (P : value -> value -> Prop) k pc e1 e2 t a1 a2,
     (forall x, P x x) ->
     env_LPequiv L P e1 e2 ->
-    eval L P pc e1 t a1 k ->
-    eval L P pc e2 t a2 k ->
+    eval L P pc e1 t k a1 -> 
+    eval L P pc e2 t k a2 -> 
     atom_LPequiv L P a1 a2.
 Proof.
-  intros L P k.
-  induction k as [| k'];
-    intros pc e1 e2 t a1 a2 Prefl He Heval1 Heval2.
-  - destruct t; unfold eval in *; subst; auto.
-    + (* TNat *)
-      destruct L; destruct pc.
-      * right. left. auto.
-      * left. auto.
-      * right. right. auto.
-      * right. right. auto.
-    + (* TVar *)
-      remember (atIndex e1 n) as o. remember (atIndex e2 n) as o'.
-      destruct o as [a |]; destruct o' as [a' |]; auto.
-      destruct a as [v1 l1]. destruct a' as [v2 l2]. subst.
-      assert (atom_LPequiv L P (Atom v1 l1) (Atom v2 l2)) by
-          (eapply list_forall2_atIndex; eauto).
-      assert (l2 = l1) by
-          (apply atom_LPequiv_lab_inv in H; auto). subst.
-      destruct pc.
-      * rewrite join_bot. assumption.
-      * rewrite join_top. destruct l1; try assumption.
-        apply atom_LPequiv_raise; assumption.
-    + (* TLam *)
-      destruct L; destruct pc.
-      * right. left. auto.
-      * left. auto.
-      * right. right. auto.
-      * right. right. auto.
-  - admit.
-Qed.
+  Admitted.
 
 Theorem non_interference :
   forall L (P : value -> value -> Prop) k pc e1 e2 t a1 a2,
     (forall x, P x x) ->
     env_LPequiv L P e1 e2 ->
-    eval L P pc e1 t a1 k ->
-    eval L P pc e2 t a2 k ->
+    eval L P pc e1 t k a1 ->
+    eval L P pc e2 t k a2 ->
     atom_Lequiv L a1 a2.
 Proof.
   intros L P k pc e1 e2 t a1 a2 Prefl He Heval1 Heval2.
